\documentclass[a4paper,11pt]{article}
\usepackage[margin=1in]{geometry}
\usepackage{enumerate}
\usepackage{xcolor}
 \usepackage{qtree}
\usepackage{fge}

\usepackage{tikz}
\usetikzlibrary{automata, positioning, arrows}
\usepackage{tikz-qtree}

\usepackage{amsmath,amsthm, amssymb, latexsym}
\usepackage{graphicx, fancyhdr}
 \usepackage{stmaryrd}
 \usepackage{mathrsfs}
\usepackage{soul}
 \usepackage[utf8]{inputenc}
\usepackage[T1]{fontenc}

\usepackage{ot-tableau}
\usepackage{multicol}

\usepackage{tipa}
\usepackage{tipx}

\usepackage[sc]{mathpazo}
\usepackage[scaled=0.95]{helvet}
\usepackage{courier}
\usepackage{tgpagella}
 
\usepackage{gb4e}

\newcommand{\powerset}{\raisebox{.15\baselineskip}{\Large\ensuremath{\wp}}}


\begin{document}

\section{Data}

\begin{exe}
\ex \gll Keng pom tus aub \\
	Keng see \textsc{Clf.sg} dog \\
\glt \textit{"Keng sees the dog."}
\end{exe}

\begin{exe}
\ex \gll Keng pom cov aub \\
	Keng see \textsc{Clf.pl} dog \\
\glt \textit{"Keng sees the dogs."} (all of the relevant dogs)
\end{exe}

\begin{exe}
\ex \gll Keng pom ib tus aub \\
	Keng see \textsc{Indef} \textsc{Clf.sg} dog \\
\glt \textit{"Keng sees a/some dog."} (non-specific)
\end{exe}

\begin{exe}
\ex \gll Keng pom ib cov aub \\
	Keng see \textsc{Indef} \textsc{Clf.pl} dog \\
\glt \textit{"Keng sees some dogs."}
\end{exe}

\begin{exe}
\ex \gll \textbf{*}Keng pom ib aub \\
	Keng sees \textsc{Indef} dog \\
\glt \textit{"Keng sees a/some dog."}
\end{exe}




\section{Proposal}

\subsection{Definites}


\begin{exe}
\ex \textbf{Cov} \textit{covers} A if: (Schwarzschild 1996) \begin{xlist}
\ex \textbf{Cov} is a set of subsets of A 
\ex Every member of A belongs to some set in \textbf{Cov} 
\ex $\emptyset$ is not in \textbf{Cov} 
\ex \textbf{Cov}(A) = $\powerset$(A), without $\emptyset$
\end{xlist}
\end{exe}

\begin{exe}
\ex $\llbracket$ cups $\rrbracket$^{M,g} = \begin{xlist}
\ex \{ \{ c_1 $\oplus$ c_2 $\oplus$ c_3 \},
\ex \{c_1 $\oplus$ c_2 \}, \{c_1 $\oplus$ c_3 \}, \{c_2 $\oplus$ c_3 \},
\ex \{c_1\}, \{c_2\}, \{c_3\} \}
\ex \textit{cups = $\powerset$(cup), without $\emptyset$}
\end{xlist}
\end{exe}

\begin{exe}
\ex $\llbracket$ \textit{tus} $\rrbracket$^{M, g} = $\lambda P\lambda x.P(x) \land AT(x)$
\end{exe}

\begin{exe}
\ex $\llbracket$ \textit{cov} $\rrbracket$^{M, g} = $\lambda P\lambda x.x \in \textbf{Cov}(P)$
\end{exe}

\begin{exe}
\ex $\llbracket$ $\iota$ $\rrbracket$ = $\lambda P: \exists x[P(x) \land \forall y[P(y) \rightarrow y \leq x]].\iota x[P(x) \land \forall y[P(y) \rightarrow y \leq x]]$
\end{exe}


\subsection{Definite compositions}

\begin{exe}
\ex Singular definite structure \\\Tree [.DP_{e} [.D^0_{\langle\langle e,t \rangle, e \rangle} $\iota$ ] [.ClfP_{\langle e,t \rangle} [.Clf^0_{\langle e, \langle e,t \rangle\rangle} \textit{tus} ] [.NP_{e} [.N^0_{e} \textit{aub} ]]]]
\end{exe}

\begin{exe}
\ex Plural definite structure \\\Tree [.DP_{e} [.D^0_{\langle\langle e,t \rangle, e \rangle} $\iota$ ] [.ClfP_{\langle e,t \rangle} [.Clf^0_{\langle e, \langle e,t \rangle\rangle} \textit{cov} ] [.NP_{e} [.N^0_{e} \textit{aub} ]]]]
\end{exe}







\subsection{Indefinites}

\begin{exe}
\ex $\llbracket$ \textit{ib} $\rrbracket$^{M, g} = $\lambda P_{\langle e,t \rangle}.f_{cf}(\lambda y.P(y) = 1)$
\end{exe}

\subsection{Contexts}

\begin{exe}
\ex \textit{AUB}_C: \{Apollo, Mars, Copper\}\begin{xlist}
	\ex\label{tusaub} \textit{tus aub} = A 
	\ex\label{ibtusaub} \textit{ib tus aub} = A or M or C 
\end{xlist}
\end{exe}


\begin{exe}
\ex\label{covselection} \textit{AUB}_C: \{Apollo, Mars, Copper\}\begin{xlist}
	\ex\label{covaub} \textit{cov aub} = AMC 
	\ex\label{ibcovaub} \textit{ib cov aub} = AMC or AM or AC or CM or A or M or C
	\ex\label{antipresup} \textit{ib cov aub} = AM or AC or CM \hspace{1cm} \textbf{(via anti-presupposition)}
\end{xlist}
\end{exe}



\pagebreak
\subsection{Indefinites composition}



Plural definite structure \\\Tree [.DP_{e} [.D^0_{\langle\langle e,t \rangle, e \rangle} $\iota$ ] [.ClfP_{\langle e,t \rangle} [.Clf^0_{\langle e, \langle e,t \rangle\rangle} \textit{cov} ] [.NP_{e} [.N^0_{e} \textit{aub} ]]]]


Plural indefinite structure \\\Tree [.DP_{\langle e,t \rangle} [.D^0_{\langle\langle e,t \rangle, \langle e,t \rangle\rangle} \textit{ib} ] [.ClfP_{\langle e,t \rangle} [.Clf^0_{\langle e, \langle e,t \rangle\rangle} \textit{cov} ] [.NP_{e} [.N^0_{e} \textit{aub} ]]]]



\begin{center}
\begin{tikzpicture}
	\node[state, initial] (0) {0:T}; 
	\node[state, right of=0, xshift=3cm] (2) {2:F}; 
	\node[state] at (1.5, 2) (1) {1:T}; 

   \draw (1) edge[right, bend left, right=0.3, ->] node{$b:F$} (2);
   \draw (0) edge[right, bend left, right=0.3, ->] node{$a:T$} (1);
   \draw (0) edge[right, bend right, right=0.3, ->] node{$b:F$} (2);
   \draw (2) edge[right, bend left, right=0.3, ->] node{$a:F$} (1);
   \draw (1) edge[loop above] node{$a:T$} (1);
   \draw (2) edge[loop below] node{$b:F$} (2);
\end{tikzpicture}
\end{center}







\section{Compositions}


\begin{exe}
\ex Composition for \textit{tus aub} \begin{xlist}
\ex $\llbracket$ \textit{tus} $\rrbracket$^{M,g} = $\lambda P\lambda x.P(x) \land AT(x)$ ~\hfill \textbf{(Lexical)}
\ex $\llbracket$ \textit{aub} $\rrbracket$^{M,g} = $\lambda x.\textsc{dog}(x)$ ~\hfill \textbf{(Lexical)}
\ex ClfP = $\llbracket$ Clf $(\llbracket$ NP $\rrbracket) \rrbracket$ ~\hfill \textbf{(FA+$\beta$-reduction)}\\
 = $\llbracket tus (\llbracket aub \rrbracket) \rrbracket$\\
 = [$\lambda P\lambda x.P(x) \land AT(x)$] \textbf{($\lambda x.\textsc{dog}(x)$)} \\
 = $\lambda x.\textsc{dog}(x) \land AT(x)$ 
\ex $\llbracket$ $\iota$ $\rrbracket$ = $\lambda P: \exists x[P(x) \land \forall y[P(y) \rightarrow y \leq x]].\iota x[P(x) \land \forall y[P(y) \rightarrow y \leq x]]$ ~\hfill \textbf{(Lexical)}
\ex DP = $\llbracket$ D $(\llbracket$ ClfP $\rrbracket) \rrbracket$ ~\hfill \textbf{(FA+$\beta$-reduction)}\\
 = $\llbracket$ $\iota$ $(\llbracket$ \textit{tus aub} $\rrbracket) \rrbracket$\\
 = $\textbf{$\lambda P$}: \exists x[\textbf{P}(x) \land \forall y[\textbf{P}(y) \rightarrow y \leq x]].\iota x[\textbf{P}(x) \land \forall y[\textbf{P}(y) \rightarrow y \leq x]]$ \\\hspace{1cm} \textbf{$(\lambda x.\textsc{dog}(x) \land AT(x))$}\\
 = $\exists x[\textbf{$(\lambda x.\textsc{dog}(x) \land AT(x))$}(x) \land \forall y[\textbf{$(\lambda x.\textsc{dog}(x) \land AT(x))$}(y) \rightarrow y \leq x]]$\\$.\iota x[\textbf{$(\lambda x.\textsc{dog}(x) \land AT(x))$}(x) \land \forall y[\textbf{$(\lambda x.\textsc{dog}(x) \land AT(x))$}(y) \rightarrow y \leq x]]$\\
\textbf{=} $\iota x[\textsc{dog}(x) \land AT(x) \land \forall y[\textsc{dog}(y) \land AT(y) \forall y \leq x ]]$ \\
\underline{defined iff:} $\exists x[\textsc{dog}(x) \land AT(x) \land \forall y[\textsc{dog}(y) \land AT(y) \rightarrow y \leq x ]]$
\end{xlist}
\end{exe}


\pagebreak
\begin{exe}
\ex Composition for \textit{cov aub} \begin{xlist} 
\ex $\llbracket$ \textit{cov} $\rrbracket$^{M,g} = $\lambda P\lambda x.P(x)$ ~\hfill \textbf{(Lexical)}
\ex $\llbracket$ \textit{aub} $\rrbracket$^{M,g} = $\lambda x.\textsc{dog}(x)$ ~\hfill \textbf{(Lexical)}
\ex ClfP = $\llbracket$ Clf $(\llbracket$ NP $\rrbracket) \rrbracket$ ~\hfill \textbf{(FA+$\beta$-reduction)}\\
 = $\llbracket cov (\llbracket aub \rrbracket) \rrbracket$\\
 = [$\lambda P\lambda x.P(x)$] \textbf{($\lambda x.\textsc{dog}(x)$)} \\
 = $\lambda x.\textsc{dog}(x)$ 
\ex $\llbracket$ $\iota$ $\rrbracket$ = $\lambda P: \exists x[P(x) \land \forall y[P(y) \rightarrow y \leq x]].\iota x[P(x) \land \forall y[P(y) \rightarrow y \leq x]]$ ~\hfill \textbf{(Lexical)}
\ex DP = $\llbracket$ D $(\llbracket$ ClfP $\rrbracket) \rrbracket$ ~\hfill \textbf{(FA+$\beta$-reduction)}\\
 = $\llbracket$ $\iota$ $(\llbracket$ \textit{cov aub} $\rrbracket) \rrbracket$\\
 = $\textbf{$\lambda P$}: \exists x[\textbf{P}(x) \land \forall y[\textbf{P}(y) \rightarrow y \leq x]].\iota x[\textbf{P}(x) \land \forall y[\textbf{P}(y) \rightarrow y \leq x]]$ \\\hspace{1cm} \textbf{$(\lambda x.\textsc{dog}(x))$}\\
 = $\exists x[\textbf{$(\lambda x.\textsc{dog}(x))$}(x) \land \forall y[\textbf{$(\lambda x.\textsc{dog}(x))$}(y) \rightarrow y \leq x]]$\\$.\iota x[\textbf{$(\lambda x.\textsc{dog}(x))$}(x) \land \forall y[\textbf{$(\lambda x.\textsc{dog}(x))$}(y) \rightarrow y \leq x]]$\\
\textbf{=} $\iota x[\textsc{dog}(x) \land \forall y[\textsc{dog}(y) \rightarrow y \leq x ]]$ \\
\underline{defined iff:} $\exists x[\textsc{dog}(x) \land \forall y[\textsc{dog}(y) \rightarrow y \leq x ]]$
\end{xlist}
\end{exe}

\begin{exe}
\ex Composition for \textit{ib tus aub} \begin{xlist}
\ex $\llbracket$ \textit{tus} $\rrbracket$^{M,g} = $\lambda P\lambda x.P(x) \land AT(x)$ ~\hfill \textbf{(Lexical)}
\ex $\llbracket$ \textit{aub} $\rrbracket$^{M,g} = $\lambda x.\textsc{dog}(x)$ ~\hfill \textbf{(Lexical)}
\ex ClfP = $\llbracket$ Clf ($\llbracket$ NP $\rrbracket$)$\rrbracket$ ~\hfill \textbf{(FA+$\beta$-reduction)}\\
= $\llbracket$ \textit{tus} ($\llbracket$ \textit{aub} $\rrbracket$)$\rrbracket$\\
= [$\lambda P\lambda x.P(x) \land AT(x)$] ($\lambda x.\textsc{dog}(x)$)\\
= $\lambda x.\textsc{dog}(x) \land AT(x)$

\ex $\llbracket$ \textit{ib} $\rrbracket$^{M,g} = $\lambda P.f_{cf}(\lambda y.P(y) = 1)$ ~\hfill \textbf{(Lexical)}
\ex DP = $\llbracket$ D ($\llbracket$ ClfP $\rrbracket$)$\rrbracket$ ~\hfill \textbf{(FA+$\beta$-reduction)}\\
= $\llbracket$ \textit{ib} ($\llbracket$ \textit{tus aub} $\rrbracket$)$\rrbracket$\\
= [$\lambda P.f_{cf}(\lambda y.P(y) = 1)$] ($\lambda x.\textsc{dog}(x) \land AT(x)$)\\
= $f_{cf}(\lambda y.(\lambda x.\textsc{dog}(x) \land AT(x))(y) = 1)$\\
= $f_{cf}.(\lambda y.\textsc{dog}(y) \land AT(y) = 1)$
\end{xlist}
\end{exe}


\begin{exe}
\ex Composition for \textit{ib cov aub} \begin{xlist}
\ex $\llbracket$ \textit{cov} $\rrbracket$^{M,g} = $\lambda P\lambda x.P(x)$ ~\hfill \textbf{(Lexical)}
\ex $\llbracket$ \textit{aub} $\rrbracket$^{M,g} = $\lambda x.\textsc{dog}(x)$ ~\hfill \textbf{(Lexical)}
\ex ClfP = $\llbracket$ Clf ($\llbracket$ NP $\rrbracket$)$\rrbracket$ ~\hfill \textbf{(FA+$\beta$-reduction)}\\
= $\llbracket$ \textit{cov} ($\llbracket$ \textit{aub} $\rrbracket$)$\rrbracket$\\
= [$\lambda P\lambda x.P(x)$] ($\lambda x.\textsc{dog}(x)$)\\
= $\lambda x.\textsc{dog}(x)$

\ex $\llbracket$ \textit{ib} $\rrbracket$^{M,g} = $\lambda P.f_{cf}(\lambda y.P(y) = 1)$ ~\hfill \textbf{(Lexical)}
\ex DP = $\llbracket$ D ($\llbracket$ ClfP $\rrbracket$)$\rrbracket$ ~\hfill \textbf{(FA+$\beta$-reduction)}\\
= $\llbracket$ \textit{ib} ($\llbracket$ \textit{cov aub} $\rrbracket$)$\rrbracket$\\
= [$\lambda P.f_{cf}(\lambda y.P(y) = 1)$] ($\lambda x.\textsc{dog}(x)$)\\
= $f_{cf}(\lambda y.(\lambda x.\textsc{dog}(x))(y) = 1)$\\
= $f_{cf}.(\lambda y.\textsc{dog}(y) = 1)$
\end{xlist}
\end{exe}







\end{document}